@prefix : <https://w3id.org/stav-eu-aia#> .
@prefix dct: <http://purl.org/dc/terms/> .
@prefix owl: <http://www.w3.org/2002/07/owl#> .
@prefix rdf: <http://www.w3.org/1999/02/22-rdf-syntax-ns#> .
@prefix xml: <http://www.w3.org/XML/1998/namespace> .
@prefix xsd: <http://www.w3.org/2001/XMLSchema#> .
@prefix rdfs: <http://www.w3.org/2000/01/rdf-schema#> .
@prefix skos: <http://www.w3.org/2004/02/skos/core#> .
@prefix stav: <https://w3id.org/stav#> .
@prefix tair: <http://tair.adaptcentre.ie/ontologies/tair/> .
@prefix stav-eu-aia: <https://w3id.org/stav-eu-aia#> .
@base <https://w3id.org/stav-eu-aia#> .

<https://w3id.org/stav-eu-aia> rdf:type owl:Ontology ;
                                owl:versionIRI <https://w3id.org/stav-eu-aia/0.1> ;
                                owl:imports <https://w3id.org/stav/0.1> ;
                                dct:creator "Arthit Suriyawongkul" ;
                                dct:description "STAV-EU-AIA represents AI system accountability concepts and relations based on the EU AI Act proposal."@en ;
                                dct:issued "2023-09-26T04:00:00"^^xsd:dateTime ;
                                dct:license "https://creativecommons.org/licenses/by/4.0/" ;
                                dct:modified "2021-09-26T04:40:00"^^xsd:dateTime ;
                                dct:publisher "ADAPT Centre, Trinity College Dublin" ;
                                dct:title "STAV-EU-AIA" ;
                                rdfs:label "STAV for European Union AI Act"@en ;
                                owl:versionInfo 0.1 .

#################################################################
#    Classes
#################################################################

###  http://tair.adaptcentre.ie/ontologies/tair/AiActRequirement
tair:AiActRequirement rdf:type owl:Class .


###  https://w3id.org/stav-eu-aia#EUAIAAIDatabaseRegisterationObligation
stav-eu-aia:EUAIAAIDatabaseRegisterationObligation rdf:type owl:Class ;
                                                   rdfs:subClassOf tair:AiActRequirement ,
                                                                   stav:RegisterationObligation ;
                                                   rdfs:label "AI Database Registeration Obligation (EU AI Act)"@en ;
                                                   skos:note """Article 51 - Registration

Before placing on the market or putting into service a high-risk AI system referred to in Article 6(2), the provider or, where applicable, the authorised representative shall register that system in the EU database referred to in Article 60.

Article 60

1. The Commission shall, in collaboration with the Member States, set up and maintain a EU database containing information referred to in paragraph 2 concerning high-risk AI systems referred to in Article 6(2) which are registered in accordance with Article 51."""@en ;
                                                   <http://www.w3.org/ns/odrl/2/source> "https://eur-lex.europa.eu/legal-content/EN/TXT/HTML/?uri=CELEX:52021PC0206&from=EN" .


###  https://w3id.org/stav-eu-aia#EUAIAQualityManagementSystemDocumentationObligation
stav-eu-aia:EUAIAQualityManagementSystemDocumentationObligation rdf:type owl:Class ;
                                                                rdfs:subClassOf tair:AiActRequirement ,
                                                                                stav:QualityManagementSystemDocumentationObligation ;
                                                                rdfs:label "Quality Management System Documentation Obligation (EU AI Act)"@en ;
                                                                skos:definition """Article 17

Providers of high-risk AI systems shall put a quality management system in place that ensures compliance with this Regulation. That system shall be documented in a systematic and orderly manner in the form of written policies, procedures and instructions, and shall include at least the following aspects:

(a) a strategy for regulatory compliance, including compliance with conformity assessment procedures and procedures for the management of modifications to the high-risk AI system;
(b) techniques, procedures and systematic actions to be used for the design, design control and design verification of the high-risk AI system;
(c) techniques, procedures and systematic actions to be used for the development, quality control and quality assurance of the high-risk AI system; 
(d) examination, test and validation procedures to be carried out before, during and after the development of the high-risk AI system, and the frequency with which they have to be carried out;
(e) technical specifications, including standards, to be applied and, where the relevant harmonised standards are not applied in full, the means to be used to ensure that the high-risk AI system complies with the requirements set out in Chapter 2 of this Title;
(f) systems and procedures for data management, including data collection, data analysis, data labelling, data storage, data filtration, data mining, data aggregation, data retention and any other operation regarding the data that is performed before and for the purposes of the placing on the market or putting into service of high-risk AI systems;
(g) the risk management system referred to in Article 9;
(h) the setting-up, implementation and maintenance of a post-market monitoring system, in accordance with Article 61;
(i) procedures related to the reporting of serious incidents and of malfunctioning in accordance with Article 62;
(j) the handling of communication with national competent authorities, competent authorities, including sectoral ones, providing or supporting the access to data, notified bodies, other operators, customers or other interested parties;
(k) systems and procedures for record keeping of all relevant documentation and information;
(l) resource management, including security of supply related measures;
(m) an accountability framework setting out the responsibilities of the management and other staff with regard to all aspects listed in this paragraph."""@en ;
                                                                <http://www.w3.org/ns/odrl/2/source> "https://eur-lex.europa.eu/legal-content/EN/TXT/HTML/?uri=CELEX:52021PC0206&from=EN" .


###  https://w3id.org/stav-eu-aia#EUAIATechnicalDocumentationObligation
stav-eu-aia:EUAIATechnicalDocumentationObligation rdf:type owl:Class ;
                                                  rdfs:subClassOf tair:AiActRequirement ,
                                                                  stav:TechnicalDocumentationObligation ;
                                                  rdfs:label "Technical Documentation Obligation (EU AI Act)"@en ;
                                                  skos:definition "The technical documentation shall be drawn up in such a way to demonstrate that the high-risk AI system compiles with the requirements set out in Chapter 2 and provide national competent authorities and notified bodies with all the necessary information to assess the compliance of the AI system with those requirements. It shall contain, at a minimum, the elements set out in Annex IV. (EU AI Act Article 11)"@en ;
                                                  skos:note "The Forum initially will be none - as Article 11 does not specify where to submit this to. Only requires it to be drawn up. But regulator can of course ask the Accountee to demonstrate. -- Should we have a property \"mustAbleToDemonstrate\" or something like that?"@en ;
                                                  <http://www.w3.org/ns/odrl/2/source> "https://eur-lex.europa.eu/legal-content/EN/TXT/HTML/?uri=CELEX:52021PC0206&from=EN" .


#################################################################
#    Individuals
#################################################################

###  http://tair.adaptcentre.ie/ontologies/tair/AiActChapter3Article18ReqColl
tair:AiActChapter3Article18ReqColl rdf:type owl:NamedIndividual ,
                                            stav-eu-aia:EUAIATechnicalDocumentationObligation .


###  http://tair.adaptcentre.ie/ontologies/tair/AiaPrReq_16.1_R1c
tair:AiaPrReq_16.1_R1c rdf:type owl:NamedIndividual ,
                                stav-eu-aia:EUAIATechnicalDocumentationObligation .


###  http://tair.adaptcentre.ie/ontologies/tair/AiaPrReq_16.1_R1f
tair:AiaPrReq_16.1_R1f rdf:type owl:NamedIndividual ,
                                stav-eu-aia:EUAIAAIDatabaseRegisterationObligation .


###  http://tair.adaptcentre.ie/ontologies/tair/AiaPrReq_51.1_R1
tair:AiaPrReq_51.1_R1 rdf:type owl:NamedIndividual ,
                               stav-eu-aia:EUAIAAIDatabaseRegisterationObligation .


###  Generated by the OWL API (version 4.5.25.2023-02-15T19:15:49Z) https://github.com/owlcs/owlapi
